Prove some useful lemmas

theories/Terms.v
@@ -1,8 +1,9 @@
+From Coq Require Import String.
 From Hammer Require Import Tactics.
 From QuickChick Require Import QuickChick.
-From Coq Require Import String.
 From LambdaST Require Import
   Eqb
+  FV
   Sets
   Types.
 
@@ -41,8 +42,7 @@ Notation "'let' '(' lhs ';' rhs ')' '=' both 'in' body" :=
 Notation "'drop' x ';' body" :=
   (TmDrop x body) (at level 97, right associativity) : term_scope.
 
-(* Can't believe I just found out you can do this: *)
-Scheme Equality for term. (* <-- no fucking way *)
+Scheme Equality for term.
 Theorem eqb_spec_term : forall a b : term, Bool.reflect (a = b) (term_beq a b).
 Proof.
   intros. destruct (term_beq a b) eqn:E; constructor;
@@ -52,6 +52,19 @@ Instance eqb_term : Eqb term := { eqb := term_beq; eq_dec := term_eq_dec; eqb_sp
 Hint Unfold term_beq : core.
 Hint Resolve term_eq_dec : core.
 Hint Resolve eqb_spec_term : core.
+
+Fixpoint fv_term e : set string :=
+  match e with
+  | TmSink | TmUnit => empty_set
+  | TmVar x => singleton_set x
+  | TmComma e1 e2 | TmSemic e1 e2 => set_union (fv_term e1) (fv_term e2)
+  | TmLetPar x y z e | TmLetCat _ x y z e => set_union (singleton_set z) (
+      set_minus (set_minus (fv_term e) (singleton_set x)) (singleton_set y))
+  | TmLet x e e' => set_union (fv_term e) (set_minus (fv_term e') (singleton_set x))
+  | TmDrop x e => set_minus (fv_term e) (singleton_set x)
+  end.
+
+Instance fv_term_inst : FV term := { fv := fv_term }.
 
 Inductive WFTerm : set string -> term -> Prop :=
   | WFTmSink : forall s,
@@ -71,29 +84,28 @@ Inductive WFTerm : set string -> term -> Prop :=
       WFTerm s (e; e')
   | WFTmLet : forall x e e' s,
       ~s x ->
-      (* is this right? *)
       WFTerm s e ->
       WFTerm (set_union s (singleton_set x)) e' ->
       WFTerm s (TmLet x e e')
   | WFTmLetPar : forall x y z e s,
-      WFTerm (set_union (set_minus s (singleton_set z)) (set_union (singleton_set x) (singleton_set y))) e ->
       s z ->
       ~s x ->
       ~s y ->
       x <> y ->
+      WFTerm (set_minus (set_union s (set_union (singleton_set x) (singleton_set y))) (singleton_set z)) e ->
       WFTerm s (TmLetPar x y z e)
   | WFTmLetCat : forall x y z e t s,
-      WFTerm (set_union (set_minus s (singleton_set z)) (set_union (singleton_set x) (singleton_set y))) e ->
       s z ->
       ~s x ->
       ~s y ->
       x <> y ->
       (* TODO: WFType s t -> *)
+      WFTerm (set_minus (set_union s (set_union (singleton_set x) (singleton_set y))) (singleton_set z)) e ->
       WFTerm s (TmLetCat t x y z e)
 .
 Hint Constructors WFTerm : core.
 
-Theorem wf_iff : forall s s' e,
+Lemma wf_set_eq : forall s s' e,
   SetEq s s' ->
   WFTerm s e ->
   WFTerm s' e.
@@ -102,3 +114,43 @@ Proof.
   generalize dependent s'.
   induction H0; cbn in *; intros; constructor; sfirstorder.
 Qed.
+
+(* TODO: it is a bit concerning that we can't prove this *)
+Lemma wf_weaken_l : forall sl sr x,
+  (forall z, fv x z -> sl z) -> (* <-- i.e., sl contains all the free variables in x *)
+  WFTerm (set_union sl sr) x ->
+  WFTerm sl x.
+Proof.
+  (*
+  intros sl sr x Hf H. remember (set_union sl sr) as s eqn:Es. generalize dependent sl. generalize dependent sr.
+  induction H; intros; subst; cbn in *.
+  - constructor.
+  - constructor.
+  - constructor. apply Hf. reflexivity.
+  - constructor; [eapply IHWFTerm1 | eapply IHWFTerm2]; sfirstorder.
+  - constructor; [eapply IHWFTerm1 | eapply IHWFTerm2]; sfirstorder.
+  - constructor; [sfirstorder | eapply IHWFTerm1; sfirstorder | eapply IHWFTerm2]; clear IHWFTerm1 IHWFTerm2.
+    admit. cbn. rewrite or_assoc.
+    shelve. shelve.
+  - constructor; [shelve | sfirstorder | sfirstorder | sfirstorder | sfirstorder].
+  - constructor; [shelve | sfirstorder | sfirstorder | sfirstorder | sfirstorder].
+  Unshelve. Abort.
+  *)
+  intros sl sr x. generalize dependent sl. generalize dependent sr. induction x; cbn in *; intros.
+  - (* sink *)
+    constructor.
+  - (* unit *)
+    constructor.
+  - (* Var id *)
+    constructor. apply H. reflexivity.
+  - (* (x1, x2) *)
+    invert H0. constructor; [eapply IHx1 | eapply IHx2]; sfirstorder.
+  - (* (x1; x2) *)
+    sinvert H0. constructor; [eapply IHx1 | eapply IHx2]; sfirstorder.
+  - (* let bind = x1 in x2 *)
+    shelve. (* sinvert H0. cbn in H7. constructor; [sfirstorder | sfirstorder |]. cbn. eapply IHx2. best. ; [eapply IHx1 | eapply IHx2]; sfirstorder. *)
+  - (* let (lhs, rhs) = bound in x *)
+    sinvert H0. constructor; [sfirstorder | sfirstorder | sfirstorder | sfirstorder |]. cbn in *.
+    eapply IHx. { shelve. } eapply wf_set_eq; [| eassumption]. cbn. intro x'. split; intro H'. { sfirstorder. }
+    destruct H'. { destruct H0. split; [| assumption]. destruct H0; [| right; assumption]. sfirstorder. }
+    split. { left. right. assumption. } intro. subst. (* Need to show that `sr` does not contain `bound` *) Abort.
